Lp2lc/Active/STLC/__Infer_umbral.lean
@@ -32,7 +32,7 @@ there is no guarantee that typeUID & valueUID will be identical, so this is the 
 class ProvingEnv where
   base: @ProvingBase F
   proofGroup : FBoundGroup F.Index (AST.Trm F)
-  proofCtx : FBoundV2 proofGroup (@InferenceWProof F base) -- TODO: need a concrete value type to save proof
+  proofCtx : FBound proofGroup (@InferenceWProof F base) -- TODO: need a concrete value type to save proof
 
 instance [env: @ProvingEnv F] : @ProvingBase F := env.base
 
